extend reduction, confluence, and typing along evar-map inclusion

theories/Logic/WP.v
@@ -133,11 +133,11 @@ constructor. intros A e Φ g. cbn. rewrite handle_inj. reflexivity.
 Qed.
 
 (**************************************************************************)
-(** *** Weakest-precondition. *)
+(** * Weakest-precondition construction. *)
 (**************************************************************************)
 
-Section WeakestPrecondition.
-  Context {E : Type -> Type} (hE : handler E).
+Section WP.
+  Context {E : Type -> Type} (h : handler E).
 
   (** Weakest-precondition functor. *)
   Program Definition wp_step (R : handler (meta E)) : handler (meta E) := {|
@@ -145,7 +145,7 @@ Section WeakestPrecondition.
       match m with
       | Ret x => fun Φ g => Φ x g
       | Bind m k => fun Φ g => R _ m (fun x g' => R _ (k x) Φ g') g
-      | Vis e => fun Φ g => hE _ e Φ g
+      | Vis e => fun Φ g => h _ e Φ g
       end
   |}.
   Next Obligation.
@@ -169,65 +169,112 @@ Section WeakestPrecondition.
       least fixpoint of [wp_step]. *)
   Definition wp : handler (meta E) := lfp wp_step.
 
+End WP.
+
+(* TODO: maybe use a better form of sealing. *)
+Arguments wp : simpl never.
+
+(**************************************************************************)
+(** * Basic lemmas about WP. *)
+(**************************************************************************)
+
+Section BasicLemmas.
+  Context {E : Type -> Type} {h : handler E}.
+
   (** Consequence rule. *)
   Lemma wp_consequence {A} {m : meta E A} {Φ Φ' g} :
     (forall x g, Φ x g -> Φ' x g) ->
-    wp _ m Φ g ->
-    wp _ m Φ' g.
+    wp h _ m Φ g ->
+    wp h _ m Φ' g.
   Proof. apply handler_mono. Qed.
 
+  (** We can change the postcondition with an equivalent one. *)
   Lemma wp_equiv {A} (m : meta E A) {Φ Φ' g} :
     (forall x g, Φ x g <-> Φ' x g) ->
-    wp _ m Φ g <-> wp _ m Φ' g.
+    wp h _ m Φ g <-> wp h _ m Φ' g.
   Proof. apply handler_equiv. Qed.
 
+  (** Unfold a single step of [wp]. Consider using [wp_Ret], [wp_Bind],
+      or [wp_Vis] instead. *)
   Lemma wp_unfold {A} {m : meta E A} {Φ g} :
-    wp _ m Φ g <-> wp_step wp _ m Φ g.
+    wp h _ m Φ g <-> wp_step h (wp h) _ m Φ g.
   Proof.
-  pose proof (H := lfp_fixpoint wp_step wp_step_mono).
+  pose proof (H := lfp_fixpoint (wp_step h) (wp_step_mono h)).
   specialize (H A m Φ g). cbn in H. rewrite H. reflexivity.
   Qed.
 
   Lemma wp_Ret {A} {x : A} {Φ g} :
-    wp _ (Ret x) Φ g <-> Φ x g.
+    wp h _ (Ret x) Φ g <-> Φ x g.
   Proof. rewrite wp_unfold. reflexivity. Qed.
 
+  Lemma wp_ret {A} (x : A) Φ g :
+    wp h _ (ret x) Φ g <-> Φ x g.
+  Proof. unfold ret. now rewrite wp_Ret. Qed.
+
   Lemma wp_Bind {A B} {m : meta E A} {f : A -> meta E B} {Φ g} :
-    wp _ (Bind m f) Φ g <-> wp _ m (fun x g' => wp _ (f x) Φ g') g.
+    wp h _ (Bind m f) Φ g <-> wp h _ m (fun x g' => wp h _ (f x) Φ g') g.
   Proof. rewrite wp_unfold. reflexivity. Qed.
 
   Lemma wp_Vis {A} {e : E A} {Φ g} :
-    wp _ (Vis e) Φ g <-> hE _ e Φ g.
+    wp h _ (Vis e) Φ g <-> h _ e Φ g.
   Proof. rewrite wp_unfold. reflexivity. Qed.
 
-  (** Induction principle on [wp]. This relies on the fact that [wp] is defined
-      as a _least_ fixpoint instead of a greatest fixpoint. *)
+  Lemma wp_trigger {A E'} `{E' -< E} (e : E' A) Φ g :
+    wp h _ (trigger e) Φ g <-> h _ (inj_event e) Φ g.
+  Proof. unfold trigger. now rewrite wp_Vis. Qed.
+
+End BasicLemmas.
+
+(** [wp] is a monotone functon from effect handlers to effect handlers. *)
+Lemma wp_mono {E} : monotone (@wp E).
+Proof.
+intros h1 h2 Hh. cbn in *. intros A m Φ g.
+induction m in Φ, g |- *.
+- rewrite !wp_Ret. firstorder.
+- rewrite !wp_Bind. intros H1. cut (wp h1 _ m (fun x g' => wp h2 _ (m0 x) Φ g') g).
+  + apply IHm.
+  + revert H1. apply wp_consequence. intros x g'. apply H.
+- rewrite !wp_Vis. apply Hh.
+Qed.
+
+(**************************************************************************)
+(** * Induction and co-induction on WP. *)
+(**************************************************************************)
+
+(** We might wonder what happens if we define [wp] as a _greatest_
+    fixpoint instead of a least fixpoint. Do we obtain a partial program logic?
+    Remarkably, we obtain the same program logic: to control whether the logic
+    is total/partial, we instead need to define the effect handler [h] as
+    a least/greatest fixpoint.
+
+    Thanks to this property we have both an induction and a coinduction
+    principle for [wp].
+*)
+
+Section Induction.
+  Context {E : Type -> Type} {h : handler E}.
+
+  (** Induction principle on [wp], aka elimination principle. *)
   Lemma wp_ind (R : handler (meta E)) :
     (forall A a Φ g, Φ a g -> R A (Ret a) Φ g) ->
     (forall A B m k Φ g, R A m (fun x g' => R B (k x) Φ g') g -> R B (Bind m k) Φ g) ->
-    (forall A e Φ g, hE A e Φ g -> R A (Vis e) Φ g) ->
-    forall A m Φ g, wp A m Φ g -> R A m Φ g.
+    (forall A e Φ g, h A e Φ g -> R A (Vis e) Φ g) ->
+    forall A m Φ g, wp h A m Φ g -> R A m Φ g.
   Proof.
-  intros Hret Hbind Hvis. apply (lfp_smallest wp_step wp_step_mono).
+  intros Hret Hbind Hvis. apply (lfp_smallest (wp_step h) (wp_step_mono h)).
   cbn. intros A [a | m k | e] Φ g ; cbn.
   - apply Hret.
   - apply Hbind.
   - apply Hvis.
   Qed.
 
-  (** We might wonder what happens if we define [wp] as a _greatest_
-      fixpoint instead of a least fixpoint. Do we obtain a partial program logic?
-      Remarkably, we obtain the same program logic: to control whether the logic
-      is total/partial, we instead need to define the effect handler [hE] as
-      a least/greatest fixpoint. *)
-
   (** Same as [wp] but as a _greatest_ fixpoint. *)
-  Definition wp' : handler (meta E) := gfp wp_step.
+  Definition wp' (h : handler E) : handler (meta E) := gfp (wp_step h).
 
   Lemma wp_unfold' {A} {m : meta E A} {Φ g} :
-    wp' _ m Φ g <-> wp_step wp' _ m Φ g.
+    wp' h _ m Φ g <-> wp_step h (wp' h) _ m Φ g.
   Proof.
-  pose proof (H := gfp_fixpoint wp_step wp_step_mono).
+  pose proof (H := gfp_fixpoint (wp_step h) (wp_step_mono h)).
   specialize (H A m Φ g). cbn in H. rewrite H. reflexivity.
   Qed.
 
@@ -236,8 +283,8 @@ Section WeakestPrecondition.
   Lemma wp_ind' (R : handler (meta E)) :
     (forall A a Φ g, Φ a g -> R A (Ret a) Φ g) ->
     (forall A B m k Φ g, R A m (fun x g' => R B (k x) Φ g') g -> R B (Bind m k) Φ g) ->
-    (forall A e Φ g, hE A e Φ g -> R A (Vis e) Φ g) ->
-    forall A m Φ g, wp' A m Φ g -> R A m Φ g.
+    (forall A e Φ g, h A e Φ g -> R A (Vis e) Φ g) ->
+    forall A m Φ g, wp' h A m Φ g -> R A m Φ g.
   Proof.
   intros Hret Hbind Hvis A m. induction m ; intros Φ g.
   - rewrite wp_unfold'. cbn. apply Hret.
@@ -247,7 +294,7 @@ Section WeakestPrecondition.
   Qed.
 
   Lemma wp_same_1 {A} (m : meta E A) Φ g :
-    wp _ m Φ g -> wp' _ m Φ g.
+    wp h _ m Φ g -> wp' h _ m Φ g.
   Proof.
   revert A m Φ g. apply wp_ind.
   - intros A a Φ g H. rewrite wp_unfold'. cbn. assumption.
@@ -256,7 +303,7 @@ Section WeakestPrecondition.
   Qed.
 
   Lemma wp_same_2 {A} (m : meta E A) Φ g :
-    wp' _ m Φ g -> wp _ m Φ g.
+    wp' h _ m Φ g -> wp h _ m Φ g.
   Proof.
   revert A m Φ g. apply wp_ind'.
   - intros A a Φ g H. rewrite wp_Ret. assumption.
@@ -267,38 +314,22 @@ Section WeakestPrecondition.
   (** This theorem justifies why we only use [wp] in the following,
       both when constructing a total and a partial program logic. *)
   Theorem wp_same {A} (m : meta E A) Φ g :
-    wp _ m Φ g <-> wp' _ m Φ g.
+    wp h _ m Φ g <-> wp' h _ m Φ g.
   Proof. split ; [apply wp_same_1 | apply wp_same_2]. Qed.
 
-  (** As a consequence of [wp_same] we get a coinduction (i.e. introduction)
-      principle for [wp]. We could probably also show this from first principles
-      without using [wp_same]. *)
+  (** Co-induction principle on [wp], aka introduction principle. *)
   Lemma wp_coind (R : handler (meta E)) :
     (forall A a Φ g, R A (Ret a) Φ g -> Φ a g) ->
     (forall A B m k Φ g, R B (Bind m k) Φ g -> R A m (fun x g' => R B (k x) Φ g') g) ->
-    (forall A e Φ g, R A (Vis e) Φ g -> hE A e Φ g) ->
-    forall A m Φ g, R A m Φ g -> wp A m Φ g.
+    (forall A e Φ g, R A (Vis e) Φ g -> h A e Φ g) ->
+    forall A m Φ g, R A m Φ g -> wp h A m Φ g.
   Proof.
-  intros Hret Hbind Hvis. setoid_rewrite wp_same. apply (gfp_greatest wp_step wp_step_mono).
-  cbn. intros A [a | m k | e] Φ g ; cbn.
+  intros Hret Hbind Hvis. setoid_rewrite wp_same.
+  apply (gfp_greatest (wp_step h) (wp_step_mono h)). cbn.
+  intros A [a | m k | e] Φ g ; cbn.
   - apply Hret.
   - apply Hbind.
   - apply Hvis.
   Qed.
 
-End WeakestPrecondition.
-
-(* TODO: maybe use a better form of sealing. *)
-Arguments wp : simpl never.
-
-(** [wp] is a monotone functon from effect handlers to effect handlers. *)
-Lemma wp_mono {E} : monotone (@wp E).
-Proof.
-intros h h' Hh. cbn in *. intros A m Φ g.
-induction m in Φ, g |- *.
-- rewrite !wp_Ret. firstorder.
-- rewrite !wp_Bind. intros H1. cut (wp h _ m (fun x g' => wp h' _ (m0 x) Φ g') g).
-  + apply IHm.
-  + revert H1. apply wp_consequence. intros x g'. apply H.
-- rewrite !wp_Vis. apply Hh.
-Qed.
+End Induction.
