theories/MetaTheory/EvarMap.v
@@ -8,6 +8,10 @@ From Metaprog Require Export Data.Evars.
     to prove that two evars maps are equal, it suffices to prove pointwise equality.
 *)
 
+(***********************************************************************)
+(** * Evar-map definition. *)
+(***********************************************************************)
+
 (** The logical view of the evar map used in proofs.
 
     We say that an evar is:
@@ -17,7 +21,12 @@ From Metaprog Require Export Data.Evars.
     - "defined" if it is present and has a definition.*)
 Definition evar_map := evar_id -> option evar_entry.
 
-(** Inclusion on (optional) evar entries. *)
+(***********************************************************************)
+(** * Inclusion on evar-maps. *)
+(***********************************************************************)
+
+(** Inclusion on (optional) evar entries. [None] means that the corresponding
+    evar is absent from the evar-map. *)
 Inductive entry_incl : option evar_entry -> option evar_entry -> Prop :=
 (** If the first evar is absent from the evar map,
     the second evar can have any entry associated to it. *)
@@ -33,12 +42,35 @@ Inductive entry_incl : option evar_entry -> option evar_entry -> Prop :=
 
 Derive Signature for entry_incl.
 
-(** Inclusion on evar maps, also written [Σ ⊑ Σ']. *)
-Definition evar_map_incl (Σ Σ' : evar_map) : Prop :=
-  forall ev, entry_incl (Σ ev) (Σ' ev).
+#[export] Instance entry_incl_Reflexive : Reflexive entry_incl.
+Proof. intros [[ty [def | ]] | ] ; constructor. Qed.
 
-Notation "Σ1 ⊑ Σ2" := (evar_map_incl Σ1 Σ2)
+#[export] Instance entry_incl_Transitive : Transitive entry_incl.
+Proof.
+intros e1 e2 e3 H1 H2. depelim H1 ; depelim H2 ; constructor.
+Qed.
+
+(** Inclusion on evar maps, also written [Σ ⊑ Σ']. *)
+Record evm_incl (Σ Σ' : evar_map) : Prop := {
+  evm_incl_prop : forall ev, entry_incl (Σ ev) (Σ' ev)
+}.
+
+Notation "Σ1 ⊑ Σ2" := (evm_incl Σ1 Σ2)
   (at level 30, no associativity).
+
+#[export] Instance evm_incl_Reflexive : Reflexive evm_incl.
+Proof. intros Σ. constructor. intros ev. reflexivity. Qed.
+
+#[export] Instance evm_incl_Transitive : Transitive evm_incl.
+Proof.
+intros Σ1 Σ2 Σ3 H1 H2. constructor. intros ev. transitivity (Σ2 ev).
+- apply H1.
+- apply H2.
+Qed.
+
+(***********************************************************************)
+(** * Basic properties of evar-maps. *)
+(***********************************************************************)
 
 (** Extensionality lemma for evar maps. *)
 Lemma evm_ext (Σ Σ' : evar_map) :
